finished copyStAux

fstar/Memory.fst
@@ -11,3 +11,7 @@ let rec read (#a : eqtype) (#b : eqtype) (mem : memory a b nat) (idr : a) (fr : 
     | Write m idw fw v -> if idw = idr && fw = fr
       then v
       else read m idr fr
+
+type memoryI a v i c = memory (a & list (either v i)) (either v i) c
+
+type idI a v i = a & list (either v i)
