fstar/StorageToMemory.fst
@@ -3,11 +3,11 @@ module StorageToMemory
 open Memory
 open Storage
 
-let rec copyStAux #v #i #a #c (mem : memory a (either v i) c) (id : a)
-  (st : structB c v i) : memory a (either v i) c
-  = match st with
-  | Mtst -> mem
-  | Store st' (Inl pf) (Var v) -> Write mem id (Inl pf) v
-  | Store st' (Inr _) v ->
+let rec copyStAux #v #i #a #c (mem : memoryI a v i c)
+  (id : idI a v i) (st : structB c v i) : Tot (memoryI a v i c) (decreases %[st; id])
+  = match st, id with
+  | Mtst, _ -> mem
+  | Store st' (Inl pf) (Var v), _ -> Write mem id (Inl pf) v
+  | Store st' (Inr x) v, (idd, xs) ->
   let copyInt = copyStAux mem id st' in
-  admit()
+  copyStAux copyInt (idd, (Inr x) :: xs) v
